a module type for SepExpr. I'm hoping that this can be used to reduce the instances   of modules and make unfolding symbols more manageable. (still wondering if modules are really right for this though, given all the headache  and the fact that most things are transparent)

src/Expr.v
@@ -639,6 +639,62 @@ Section env.
 
 End env.
 
+Section exists_subst.
+  Variable types : list type.
+  Variable funcs : functions types.
+  Variable U1 : env types.
+  
+  (* Unification variables corresponding to genuine Coq existentials *)
+  Fixpoint exists_subst (CU : env types)
+    (U : list (tvar * option (expr types)))
+    : (env types -> Prop) -> Prop :=
+    match U as U with
+      | nil => fun cc => cc nil
+      | (t,v) :: r => fun cc =>
+        match v with
+          | None => 
+            exists v : tvarD types t, exists_subst (match CU with
+                                                      | nil => nil
+                                                      | _ :: CU' => CU'
+                                                    end) r (fun z => cc (existT _ t v :: z))
+          | Some v => 
+            match exprD funcs CU U1 v t with
+              | None => False
+              | Some v1 =>
+                match CU with
+                  | nil => exists_subst nil r (fun z => cc (existT _ t v1 :: z))
+                  | existT t' v' :: CU' =>
+                    match exprD funcs CU U1 v t' with
+                      | None => False
+                      | Some v'' => v' = v'' /\ exists_subst CU' r (fun z => cc (existT _ t v1 :: z))
+                    end
+                end
+            end
+        end
+    end.
+
+Lemma exists_subst_exists : forall CU
+  (B : list (tvar * option (expr types))) P,
+  exists_subst CU B P ->
+  exists C, P C.
+Proof.
+(*
+      clear. induction B; simpl; intros.
+      eauto.
+      destruct a; simpl in *. destruct o.
+      destruct (exprD funcs CU A e t); try tauto.
+      eapply IHB in H; destruct H; eauto. 
+      destruct H. eapply IHB in H. destruct H; eauto.
+    Qed.
+*)
+Admitted.
+
+End exists_subst.
+
+
+
+
+
 Implicit Arguments Const [ types t ].
 Implicit Arguments Var [ types ].
 Implicit Arguments UVar [ types ].
