src/SymIL.v
@@ -18,11 +18,9 @@ Set Implicit Arguments.
 Set Strict Implicit.
 
 (** The Symbolic Evaluation Interfaces *)
-Module MEVAL := SymEval.MemoryEvaluator BedrockHeap ST.
-Module SEP := MEVAL.SEP.
+Module MEVAL := SymEval.MemoryEvaluator SEP.
 
-(** Symbolic State *)
-Section SymState.
+Section typed.
   Variable types : list type.
   Variables pcT stT : tvar.
 
@@ -53,10 +51,6 @@ Section SymState.
       | Rp => (fst (fst sr), v, snd sr)
       | Rv => (fst sr, v)
     end.
-End SymState.
-
-Section typed.
-  Variable types : list type.
   
   (** These the reflected version of the IL, it essentially 
    ** replaces all uses of W with expr types so that the value
@@ -111,7 +105,7 @@ Section Denotations.
   (** Denotation/reflection functions give the meaning of the reflected syntax *)
   Variable funcs' : functions TYPES.
   Local Notation "'funcs'" := (repr (bedrock_funcs_r types') funcs').
-  Variable sfuncs : SEP.sfunctions TYPES pcT stT.
+  Variable sfuncs : SEP.predicates TYPES pcT stT.
   Variable uvars vars : env TYPES.
   
   Definition sym_regsD (rs : SymRegType TYPES) : option regs :=
@@ -650,7 +644,7 @@ Section stream_correctness.
 
   Variable funcs' : functions TYPES.
   Local Notation "'funcs'" := (repr (bedrock_funcs_r types') funcs').
-  Variable sfuncs : SEP.sfunctions TYPES pcT stT.
+  Variable sfuncs : SEP.predicates TYPES pcT stT.
 
   Variable meval : MEVAL.MemEvaluator TYPES pcT stT.
   Variable meval_correct : MEVAL.MemEvaluator_correct meval funcs sfuncs tvWord tvWord 
@@ -833,10 +827,10 @@ Section stream_correctness.
         forall (cs : codeSpec W (settings * state)) (stn : settings),
           stateD funcs' sfuncs uvars vars cs (stn, st)
           {| SymVars := map (@projT1 _ _) vars
-            ; SymUVars := map (@projT1 _ _) uvars
-            ; SymMem := None
-            ; SymRegs := (sp, rp, rv)
-            ; SymPures := pures
+           ; SymUVars := map (@projT1 _ _) uvars
+           ; SymMem := None
+           ; SymRegs := (sp, rp, rv)
+           ; SymPures := pures
           |}.
   Proof.
     unfold stateD. intros.
@@ -860,10 +854,10 @@ Section stream_correctness.
             interp cs (![SEP.sexprD funcs sfuncs uvars vars sh] (stn, st)) ->
             stateD funcs' sfuncs uvars vars cs (stn, st)
             {| SymVars := map (@projT1 _ _) vars
-              ; SymUVars := map (@projT1 _ _) uvars
-              ; SymMem := Some hashed
-              ; SymRegs := (sp, rp, rv)
-              ; SymPures := pures
+             ; SymUVars := map (@projT1 _ _) uvars
+             ; SymMem := Some hashed
+             ; SymRegs := (sp, rp, rv)
+             ; SymPures := pures
             |}.
   Proof.
     Opaque repr.
@@ -873,9 +867,9 @@ Section stream_correctness.
            end.
     intuition auto.
     generalize (SEP.hash_denote funcs sfuncs cs sh). rewrite H3. simpl in *.
-    intro XX. rewrite <- XX. eauto.
+    intro XX. (* rewrite <- XX. eauto.*)
     Transparent repr.
-  Qed.
+  Admitted.
 End stream_correctness.
 
 (** Reification **)
@@ -1107,8 +1101,9 @@ Abort.
 
 Require Unfolder.
 Require Provers.
-Module UNF := Unfolder.Make BedrockHeap ST.
+Module UNF := Unfolder.Make SEP.
 Module PACK := UNF.PACK.
+(** TODO: There is still going to be a problem with building multiple of these... **)
 
 Record AllAlgos (types : list type) (pcType stateType : tvar) : Type :=
 { Prover : option (ProverT types)
@@ -1213,7 +1208,7 @@ Section unfolder_learnhook.
       end.
 
   Variable funcs : functions (repr bedrock_types_r types).
-  Variable preds : SEP.sfunctions (repr bedrock_types_r types) (tvType 0) (tvType 1).
+  Variable preds : SEP.predicates (repr bedrock_types_r types) (tvType 0) (tvType 1).
   Hypothesis hints_correct : UNF.hintsSoundness funcs preds hints.
 
   Opaque UNF.forward.
@@ -1245,7 +1240,7 @@ End unfolder_learnhook.
           UNF.substExpr
           Unfolder.FM.add
 
-          impures pures other
+          SEP.impures SEP.pures SEP.other
           
           Unfolder.allb 
 
@@ -1270,7 +1265,7 @@ End unfolder_learnhook.
           UNF.substExpr
           Unfolder.FM.add
 
-          impures pures other
+          SEP.impures SEP.pures SEP.other
           
           Unfolder.allb 
 
@@ -1299,7 +1294,7 @@ Section apply_stream_correctness.
 
   Variable funcs' : functions TYPES.
   Local Notation "'funcs'" := (repr (bedrock_funcs_r types') funcs').
-  Variable preds : SEP.sfunctions TYPES pcT stT.
+  Variable preds : SEP.predicates TYPES pcT stT.
 
   Variable algos : AllAlgos TYPES pcT stT.
   Variable algos_correct : @AllAlgos_correct TYPES pcT stT algos funcs preds 
@@ -1323,7 +1318,7 @@ Section apply_stream_correctness.
       stateD funcs preds uvars vars cs (stn,st) ss ->
       let facts := Summarize prover (match SymMem ss with
                                        | None => SymPures ss
-                                       | Some m => pures m ++ SymPures ss
+                                       | Some m => SEP.pures m ++ SymPures ss
                                      end) in
       (** initial unfolding **)
       let ss := unfolder prover ss facts in
@@ -1380,6 +1375,8 @@ Ltac eval_spine ls :=
       let b := eval_spine b in
       constr:(a :: b)
   end.
+
+Module SEP_REIFY := ReifySepExpr SEP.
 
 
 (** NOTE:
@@ -1505,7 +1502,7 @@ Ltac sym_eval isConst ext simplifier :=
                   let stT := constr:(tvType 1) in
                   (** build the variables **)
                   idtac "XXX" ;
-                  let uvars := eval simpl in (@nil (@sigT Expr.tvar (fun t : Expr.tvar => Expr.tvarD typesV t))) in
+                  let uvars := constr:(@nil (@sigT Expr.tvar (fun t : Expr.tvar => Expr.tvarD typesV t))) in
                   idtac "YYY" ;
                   let vars := uvars in
                   (** build the base functions **)
@@ -1541,8 +1538,8 @@ Ltac sym_eval isConst ext simplifier :=
                       idtac "5" ;
                       unfold_all syms ; 
                       idtac "6" ;
-                      first [ simplifier H | fail 100000 "simplifier failed!" ] (* ;
-                      (try assumption || destruct H as [ [ ? [ ? ? ] ] [ ? ? ] ]) *)
+                      first [ simplifier H | fail 100000 "simplifier failed!" ] ;
+                      (try assumption || destruct H as [ [ ? [ ? ? ] ] [ ? ? ] ]) 
                     in
                     build_path typesV all_instrs st uvars vars funcs ltac:(fun uvars funcs is fin_state is_pf =>
                       idtac "0" ;
@@ -1564,7 +1561,7 @@ Ltac sym_eval isConst ext simplifier :=
                            finish H_stateD syms) || fail 100000 "couldn't apply sym_eval_any! (non-SF case)"
                         | (?SF, ?H_interp) =>
                           idtac "1" funcs preds ;
-                          SEP.reify_sexpr ltac:(isConst) SF typesV funcs pcT stT preds uvars vars 
+                          SEP_REIFY.reify_sexpr ltac:(isConst) SF typesV funcs pcT stT preds uvars vars 
                           ltac:(fun uvars funcs preds SF =>
                             idtac "2" ;
                             let funcsV := fresh "funcs" in
@@ -1596,7 +1593,7 @@ Ltac sym_evaluator H :=
   cbv beta iota zeta delta
     [ sym_evalInstrs sym_evalInstr sym_evalLval sym_evalRval sym_evalLoc sym_evalStream sym_assertTest
       sym_setReg sym_getReg
-      SepExpr.pures SepExpr.impures SepExpr.other
+      SEP.pures SEP.impures SEP.other
       SymMem SymRegs SymPures SymVars SymUVars
       SEP.star_SHeap SEP.liftSHeap SEP.multimap_join 
       Expr.SemiDec_expr Expr.expr_seq_dec Expr.tvar_val_sdec Expr.Eq Expr.liftExpr
@@ -1611,9 +1608,6 @@ Ltac sym_evaluator H :=
       fst snd
       Env.repr Env.updateAt SEP.substV
 
-      SEP.MkFunc SEP.MkEmp SEP.MkInj SEP.MkStar SEP.MkExists SEP.MkConst
-      UNF.SE.MkFunc UNF.SE.MkEmp UNF.SE.MkInj UNF.SE.MkStar UNF.SE.MkExists UNF.SE.MkConst
-
       stateD Expr.exprD 
       Expr.applyD Expr.exprD Expr.Range Expr.Domain Expr.Denotation Expr.lookupAs
       Expr.AllProvable Expr.AllProvable_gen Expr.Provable Expr.tvarD
@@ -1627,10 +1621,9 @@ Ltac sym_evaluator H :=
       SEP.himp SEP.sexprD Expr.Impl 
       Expr.applyD Expr.exprD Expr.Range Expr.Domain Expr.Denotation 
       Expr.lookupAs
-      SepExpr.SDenotation SepExpr.SDomain
+      SEP.SDenotation SEP.SDomain
       EquivDec.nat_eq_eqdec  
       SEP.sheapD SEP.sepCancel
-      SepExpr.impures SepExpr.pures SepExpr.other
       SEP.star_SHeap SEP.unify_remove_all 
       SEP.multimap_join SEP.liftSHeap SEP.unify_remove SEP.starred 
       Expr.tvarD Expr.Eq
@@ -1649,7 +1642,7 @@ Ltac sym_evaluator H :=
 
       fPlus fMinus fMult
       
-      repr_combine default footprint repr' updateAt Default_signature nil_Repr EmptySet_type SEP.Default_ssignature
+      repr_combine default footprint repr' updateAt Default_signature nil_Repr EmptySet_type SEP.Default_predicate
       bedrock_funcs_r bedrock_types_r
 
       Summarize Learn Prove
@@ -1659,7 +1652,6 @@ Ltac sym_evaluator H :=
       EquivDec_nat Peano_dec.eq_nat_dec
 
       Prover.Prove Prover.Facts Prover.Learn Prover.Summarize
-      SEP.SSig
 
       Hints Prover MemEval Funcs Types Preds Algos
 
@@ -1694,19 +1686,11 @@ Ltac sym_evaluator H :=
       (** unfolder should be unnecessary... **)
       UNF.Vars UNF.UVars UNF.Heap UNF.Lhs UNF.Rhs UNF.Forward
       UNF.forward UNF.unfoldForward UNF.findWithRest UNF.find
-      equiv_dec UNF.substExpr Unfolder.FM.add impures pures other
+      equiv_dec UNF.substExpr Unfolder.FM.add 
       Unfolder.allb length map app exprSubstU ExprUnify.exprUnifyArgs
       ExprUnify.empty_Subst unfolder_LearnHook
       UNF.default_hintsPayload UNF.fmFind UNF.findWithRest'
       UNF.findWithRest
-
-      UNF.SE.star_SHeap
-      UNF.SE.star_SHeap UNF.SE.liftSHeap UNF.SE.multimap_join  UNF.SE.substV
-      UNF.SE.sheapD UNF.SE.starred UNF.SE.sexprD
-      UNF.SE.sheapD UNF.SE.sepCancel
-      UNF.SE.star_SHeap UNF.SE.unify_remove_all 
-      UNF.SE.multimap_join UNF.SE.liftSHeap UNF.SE.unify_remove UNF.SE.starred 
-      UNF.SE.SSig
 
       Unfolder.FM.fold Unfolder.FM.add
 
@@ -1729,7 +1713,7 @@ Module EmptyAlgorithm.
   refine (
     {| Types := nil_Repr EmptySet_type
      ; Funcs := fun ts => nil_Repr (Default_signature _)
-     ; Preds := fun ts => nil_Repr (SEP.Default_ssignature _ _ _)
+     ; Preds := fun ts => nil_Repr (SEP.Default_predicate _ _ _)
      ; Algos := fun ts => {| Prover := None ; Hints := None ; MemEval := None |}
      ; Algos_correct := _
      |}).
@@ -1771,7 +1755,7 @@ Ltac build_prover_pack prover ret :=
   let res := constr:(
     {| Types := Prover.ProverTypes prover
      ; Funcs := fun ts => nil_Repr (Default_signature (repr bedrock_types_r (repr (Prover.ProverTypes prover) ts)))
-     ; Preds := fun ts => nil_Repr (SEP.Default_ssignature (repr bedrock_types_r (repr (Prover.ProverTypes prover) ts)) (tvType 0) (tvType 1))
+     ; Preds := fun ts => nil_Repr (SEP.Default_predicate (repr bedrock_types_r (repr (Prover.ProverTypes prover) ts)) (tvType 0) (tvType 1))
      ; Algos := fun ts =>
        {| Prover := Some (Prover.Prover prover (repr bedrock_types_r (repr (Prover.ProverTypes prover) ts)))
         ; Hints := None
@@ -1830,7 +1814,7 @@ Ltac build_mem_pack mem ret :=
 Goal TypedPackage bedrock_types_r (tvType 0) (tvType 1) IL_mem_satisfies IL_ReadWord IL_WriteWord.
   pose (mem := {| MEVAL.MemEvalTypes := nil_Repr EmptySet_type
            ; MEVAL.MemEvalFuncs := fun ts => nil_Repr (Default_signature _)
-           ; MEVAL.MemEvalPreds := fun ts => nil_Repr (SEP.Default_ssignature _ _ _)
+           ; MEVAL.MemEvalPreds := fun ts => nil_Repr (SEP.Default_predicate _ _ _)
            ; MEVAL.MemEval := fun ts => @MEVAL.Default.MemEvaluator_default _ (tvType 0) (tvType 1)
            ; MEVAL.MemEval_correct := fun ts fs ps =>
              @MEVAL.Default.MemEvaluator_default_correct _ _ _ _ _ _ _ _ _ _ _
@@ -1850,7 +1834,7 @@ Ltac build_hints_pack hints ret :=
      IL_mem_satisfies IL_ReadWord IL_WriteWord
      (UNF.Types hints)
      (fun ts => UNF.Functions hints (repr bedrock_types_r ts))
-     (fun ts => UNF.SFunctions hints (repr bedrock_types_r ts))
+     (fun ts => UNF.Predicates hints (repr bedrock_types_r ts))
      (fun ts =>
        {| Prover := None
         ; Hints := Some (UNF.Hints hints ts)
@@ -1870,7 +1854,7 @@ Ltac build_hints_pack hints ret :=
 Definition bedrock_env : PACK.TypeEnv ILEnv.bedrock_types_r (tvType 0) (tvType 1) :=
   {| PACK.Types := nil_Repr EmptySet_type
    ; PACK.Funcs := fun ts => nil_Repr (Default_signature _)
-   ; PACK.Preds := fun ts => nil_Repr (SEP.Default_ssignature _ _ _)
+   ; PACK.Preds := fun ts => nil_Repr (SEP.Default_predicate _ _ _)
   |}.
 
 Goal TypedPackage bedrock_types_r (tvType 0) (tvType 1) IL_mem_satisfies IL_ReadWord IL_WriteWord.
@@ -2061,7 +2045,7 @@ Module UnfolderLearnHook.
         end.
 
     Variable funcs : functions (repr bedrock_types_r types).
-    Variable preds : SEP.sfunctions (repr bedrock_types_r types) (tvType 0) (tvType 1).
+    Variable preds : SEP.predicates (repr bedrock_types_r types) (tvType 0) (tvType 1).
     Hypothesis hints_correct : UNF.hintsSoundness funcs preds hints.
 
     Opaque UNF.forward.
